Alphabet_Scene_Space_Examples.thy
@@ -1,0 +1,47 @@
+section \<open> Example Alphabet Scene Spaces \<close>
+
+theory Alphabet_Scene_Space_Examples
+imports Alphabet_Scene_Spaces
+begin
+
+alphabet test = 
+  x :: bool
+  y :: nat 
+  z :: "int list"
+
+alphabet_scene_space test
+
+term "\<lbrace>x, y, z\<rbrace>"
+
+lemma "z \<in>\<^sub>F \<lbrace>x, y, z\<rbrace>"
+  by simp
+
+lemma "UNIV\<^sub>F(test) = \<lbrace>x, y, z\<rbrace>"
+  by (simp add: frame)
+
+alphabet test2 = test +
+  u :: string
+  v :: int
+
+alphabet_scene_space test2
+
+lemma "UNIV\<^sub>F(test2) = \<lbrace>x, y, z, u, v\<rbrace>"
+  by (simp add: frame)
+
+alphabet test3 = test2 +
+  w :: string
+
+alphabet_scene_space test3
+
+lemma "UNIV\<^sub>F(test3) = \<lbrace>x, y, z, u, v, w\<rbrace>"
+  by (simp add: frame)
+
+alphabet test4 = test3 +
+  j :: string
+
+alphabet_scene_space test4
+
+lemma "UNIV\<^sub>F(test4) = \<lbrace>x, y, z, u, v, w, j\<rbrace>"
+  by (simp add: frame)
+
+end
