Alphabet_Scene_Spaces.thy
@@ -1,0 +1,127 @@
+section \<open> Alphabet Scene Spaces \<close>
+
+theory Alphabet_Scene_Spaces
+  imports Frames
+  keywords "alphabet_scene_space" :: "thy_defn"
+begin
+
+text \<open> The scene space for an alphabet is constructed using the set of scenes corresponding to
+  each lens, the base lens, and the more lens, to allow for extension. \<close>
+
+definition alpha_scene_space :: "'s scene list \<Rightarrow> ('b::scene_space \<Longrightarrow> 's) \<Rightarrow> 's scene list" where
+"alpha_scene_space xs m\<^sub>L = xs @ map (\<lambda> x. x ;\<^sub>S m\<^sub>L) Vars"
+
+definition alpha_scene_space' :: "'s scene list \<Rightarrow> ('b::scene_space \<Longrightarrow> 's) \<Rightarrow> ('c \<Longrightarrow> 's) \<Rightarrow> 'c scene list" where
+"alpha_scene_space' xs m\<^sub>L p\<^sub>L = alpha_scene_space (map (\<lambda> x. x /\<^sub>S p\<^sub>L) xs) (m\<^sub>L /\<^sub>L p\<^sub>L)"
+
+lemma mem_alpha_scene_space_iff [simp]: 
+  "x \<in> set (alpha_scene_space xs m\<^sub>L) \<longleftrightarrow> (x \<in> set xs \<or> x \<in> (\<lambda> x. x ;\<^sub>S m\<^sub>L) ` set Vars)"
+  by (simp add: alpha_scene_space_def)
+
+lemma alpha_scene_space_class_intro:
+  assumes 
+    "\<forall> x\<in>set xs. idem_scene x"
+    "scene_indeps (set xs)"
+    "vwb_lens m\<^sub>L" \<comment> \<open> The more lens \<close>
+    "\<forall> x\<in>set xs. x \<bowtie>\<^sub>S \<lbrakk>m\<^sub>L\<rbrakk>\<^sub>\<sim>"  
+    "(foldr (\<squnion>\<^sub>S) xs \<lbrakk>m\<^sub>L\<rbrakk>\<^sub>\<sim>) = \<top>\<^sub>S"
+  shows "class.scene_space (alpha_scene_space xs m\<^sub>L)"
+proof (simp add: alpha_scene_space_def, unfold_locales)
+  show "\<And>x. x \<in> set (xs @ map (\<lambda>x. x ;\<^sub>S m\<^sub>L) Vars) \<Longrightarrow> idem_scene x"
+    using assms(1) idem_scene_Vars by fastforce
+  show "scene_indeps (set (xs @ map (\<lambda>x. x ;\<^sub>S m\<^sub>L) Vars))"
+    apply (auto simp add: scene_indeps_def pairwise_def)
+    apply (metis assms(2) pairwiseD scene_indeps_def)
+    using assms(1) assms(4) idem_scene_Vars scene_comp_pres_indep apply blast
+    using assms(1) assms(4) idem_scene_Vars scene_comp_pres_indep scene_indep_sym apply blast
+    apply (metis indep_Vars pairwiseD scene_comp_indep scene_indeps_def)
+    done
+  show "scene_span (xs @ map (\<lambda>x. x ;\<^sub>S m\<^sub>L) Vars)"
+    apply (simp add: scene_span_def)
+    apply (subst foldr_compat_dist)
+    apply (simp)
+    apply (metis assms(3) assms(5) scene_comp_top_scene scene_span_def span_Vars)    
+    done
+qed
+
+lemma alpha_scene_space_class_intro':
+  assumes 
+    "\<forall> x\<in>set xs. idem_scene x"
+    "scene_indeps (set xs)"
+    "vwb_lens m\<^sub>L" \<comment> \<open> The more lens \<close>
+    "vwb_lens p\<^sub>L" \<comment> \<open> The parent more lens \<close>
+    "m\<^sub>L \<subseteq>\<^sub>L p\<^sub>L"
+    "\<forall>a\<in>set xs. a \<subseteq>\<^sub>S \<lbrakk>p\<^sub>L\<rbrakk>\<^sub>\<sim>"
+    "\<forall> x\<in>set xs. x \<bowtie>\<^sub>S \<lbrakk>m\<^sub>L\<rbrakk>\<^sub>\<sim>"
+    "(foldr (\<squnion>\<^sub>S) xs \<lbrakk>m\<^sub>L\<rbrakk>\<^sub>\<sim>) = \<lbrakk>p\<^sub>L\<rbrakk>\<^sub>\<sim>"
+  shows "class.scene_space (alpha_scene_space' xs m\<^sub>L p\<^sub>L)"
+  unfolding alpha_scene_space'_def
+  apply (rule alpha_scene_space_class_intro)
+      apply (simp_all add: assms scene_quotient_idem)
+  apply (simp add: scene_indeps_def pairwise_def )
+  apply (metis assms(2) pairwiseD scene_indeps_def scene_quotient_indep)
+  using assms(3) assms(4) assms(5) lens_quotient_vwb apply blast
+   apply (simp add: assms lens_scene_quotient scene_quotient_indep)
+  apply (subst foldr_scene_union_add_tail[THEN sym])
+  apply (simp)
+  apply (metis (mono_tags, lifting) assms(2) pairwiseD pairwise_imageI scene_indep_compat scene_indeps_def scene_quotient_indep)
+  apply (simp add: assms(4) assms(5) assms(7) lens_scene_quotient scene_quotient_indep)
+  apply (subst foldr_compat_quotient_dist)
+  apply (metis assms(2) pairwise_alt scene_indep_compat scene_indeps_def)
+  using assms(6) apply blast
+  apply (simp add: lens_scene_quotient assms)
+  apply (subst scene_union_quotient[THEN sym])
+  apply (metis assms(2) assms(3) assms(4) assms(5) assms(7) assms(8) bot_idem_scene empty_iff foldr.simps(1) foldr_scene_union_add_tail id_apply list.set(1) order_eq_refl pairwise_compat_foldr pairwise_empty pairwise_mono scene_bot_least scene_indep_compat scene_indeps_def scene_union_incompat sublens'_implies_subscene sublens_implies_sublens' subscene_antisym)
+  apply (metis assms(2) assms(6) foldr_scene_indep pairwise_def scene_indep_compat scene_indep_sym scene_indeps_def scene_le_iff_indep_inv)
+  apply (simp add: assms(3) assms(4) assms(5) sublens'_implies_subscene sublens_implies_sublens')
+  apply (subst foldr_scene_union_add_tail)
+  apply (metis assms(2) pairwiseD pairwiseI scene_indep_compat scene_indeps_def)
+  using assms(7) scene_indep_compat apply blast
+  apply (simp add: assms(8))
+  apply (metis assms(4) scene_comp_quotient scene_comp_top_scene)
+  done
+  
+definition more_frame :: "('a::scene_space \<Longrightarrow> 'b::scene_space) \<Rightarrow> 'b frame" where
+"more_frame m\<^sub>L = \<Union>\<^sub>F ((\<lambda>x. \<lbrakk>x ;\<^sub>S m\<^sub>L\<rbrakk>\<^sub>F) ` set Vars)"
+
+lemma more_frame_unit [simp]: "more_frame (m\<^sub>L :: unit \<Longrightarrow> 'b::scene_space) = \<lbrace>\<rbrace>"
+  by (simp add: more_frame_def)
+
+named_theorems scene_space_defs
+
+lemmas scene_space_lemmas =
+   lens_plus_scene[THEN sym] lens_equiv_scene[THEN sym] lens_equiv_sym
+   lens_scene_comp[THEN sym] lens_quotient_vwb lens_quotient_comp
+   comp_vwb_lens lens_comp_assoc[THEN sym] sublens_iff_subscene[THEN sym] 
+   lens_scene_quotient[THEN sym] sublens_greatest lens_quotient_id_denom
+   scene_comp_assoc lens_quotient_indep lens_quotient_plus[THEN sym] lens_quotient_bij 
+   plus_pred_sublens lens_scene_top_iff_bij_lens
+
+method basis_lens uses defs =
+  (rule basis_lens_intro, simp_all add: scene_space_defs alpha_scene_space_def alpha_scene_space'_def scene_space_lemmas)
+
+method more_frame = 
+  ((simp add: frame_scene_top frame_scene_foldr)?
+  ,(simp_all add: frame_scene_top frame_scene_foldr alpha_scene_space'_def alpha_scene_space_def scene_space_lemmas more_frame_def scene_space_defs image_comp))
+
+method alpha_scene_space = 
+  (rule scene_space_class.intro
+  ,(intro_classes)[1]
+  ,simp add: scene_space_defs lens_scene_quotient
+  ,rule alpha_scene_space_class_intro alpha_scene_space_class_intro'
+  ,simp_all add: scene_indeps_def pairwise_def scene_space_lemmas)
+
+ML_file \<open>Alphabet_Scene_Spaces.ML\<close>
+
+ML \<open>
+
+val _ =
+  Outer_Syntax.command @{command_keyword alphabet_scene_space} "define a scene space for an alphabet"
+    (Parse.name
+    >> (fn n =>
+        Toplevel.theory (Alphabet_Scene_Spaces.mk_alpha_scene_space n)));
+
+
+\<close>
+
+end
